new/golang/theory/vmap.v
@@ -1,9 +1,34 @@
 From Perennial.goose_lang Require Import proofmode lifting.
 From New.golang.defn Require Export vmap.
 From New.golang.theory Require Import list.
+From stdpp Require Import sorting.
 
 Section wps.
 Context `{sem: ffi_semantics} `{!ffi_interp ffi} `{!heapGS Σ}.
+
+Local Instance cmp_trans : Transitive vmap.vmap.cmp.
+Proof.
+  intros [][][]??. simpl in *.
+  unfold is_true in *. rewrite !Pos.leb_le in H H0 *. lia.
+Qed.
+
+Local Instance cmp_total : Total vmap.vmap.cmp.
+Proof.
+  intros [][]. simpl in *.
+  unfold is_true in *. rewrite !Pos.leb_le. lia.
+Qed.
+
+Search map_to_list.
+
+Local Lemma Sorted_unique l1 l2 :
+  NoDup l1.*1 →
+  NoDup l2.*1 →
+  Sorted (vmap.vmap.cmp) l1 →
+  Sorted (vmap.vmap.cmp) l2 →
+  l1 ≡ₚ l2 →
+  l1 = l2.
+Proof.
+Admitted.
 
 (* XXX: this is a "pure" step. *)
 Lemma wp_vmap_Insert (k v : val) (m : gmap val val) :
@@ -17,7 +42,7 @@ Proof.
     wp_rec. wp_pures.
     wp_apply (wp_list_Match).
     wp_pures.
-    rewrite /vmap.val_def /vmap.vmap.val_list_def insert_empty map_fold_singleton /=.
+    rewrite /vmap.val_def /vmap.vmap.val_list_def insert_empty map_to_list_singleton /=.
     by iApply "HΦ".
   - iIntros (?) "_ HΦ".
     wp_rec. wp_pures.
@@ -27,55 +52,57 @@ Proof.
     destruct l eqn:Hl.
     { exfalso. subst l.
       rewrite /vmap.vmap.val_list_def /= in Hl.
-      apply fmap_nil_inv in Hl.
-      rewrite /map_fold /gmap_fold /= in Hl.
-      rewrite map_fold_insert_L in Hl; last done.
-      {
-        apply (f_equal length) in Hl.
-        rewrite /vmap.insert_replace_sorted /= in Hl.
-        set y:=(map_fold _ _ _) in Hl.
-        destruct y.
-        { done. }
-        { destruct p, (val_le i v0), (val_le v0 i); done. }
-      }
-      intros.
-      induction y.
-      {
-        simpl. destruct (val_le j1 j2) eqn:Hy, (val_le j2 j1) eqn:Hx.
-        - exfalso. unfold val_le in *.
-          rewrite !Pos.leb_le in Hx, Hy.
-          pose proof (Pos.le_antisym _ _ Hx Hy).
-          apply (f_equal (decode (A:=val))) in H3.
-          rewrite !decode_encode in H3.
-          inversion H3. subst. done.
-        - done.
-        - done.
-        - exfalso.
-          rewrite !Positive_as_OT.leb_nle in Hx Hy.
-          pose proof (Pos.le_total (encode j1) (encode j2)) as [|].
-          + by apply Hx.
-          + by apply Hy.
-      }
-      {
-        destruct a. simpl in *.
-        destruct (val_le j1 j2) eqn:Hy, (val_le j2 j1) eqn:Hx,
-                   (val_le j1 v0) eqn:?, (val_le j2 v0) eqn:?,
-                     (val_le v0 j1) eqn:?, (val_le v0 j2) eqn:?;
-        unfold val_le in *; simpl in *;
-          repeat lazymatch goal with
-          | [ H : context [Pos.leb] |- _ ] => rewrite ?H; rewrite ?Pos.leb_le ?Pos.leb_gt in H
-          end;
-          repeat lazymatch goal with
-            | [ H1 : Pos.le ?a ?b , H2 : Pos.le ?b ?a |- _ ] =>
-                let Htmp := fresh in
-                pose proof (Pos.le_antisym _ _ H1 H2) as Htmp; clear H1 H2;
-                apply (f_equal (decode (A:=val))) in Htmp;
-                rewrite !decode_encode in Htmp; injection Htmp as ->
-            end.
-        all: try (reflexivity || lia || by exfalso).
-      }
+      apply fmap_nil_inv, (f_equal length) in Hl.
+      erewrite (Permutation_length ltac:(eapply merge_sort_Permutation)) in Hl.
+      by rewrite map_to_list_length map_size_insert H /= in Hl.
     }
-    admit.
+    wp_pures.
+    subst l.
+    rewrite /vmap.val_list_def /= in Hl.
+    apply fmap_cons_inv in Hl as [[] [? [-> [ -> Hl]]]]. subst.
+    wp_pures.
+    wp_if_destruct.
+    {
+      wp_pures.
+      wp_if_destruct.
+      - apply Pos.leb_le in Heqb, Heqb0.
+        pose proof (Pos.le_antisym _ _ Heqb Heqb0) as Heq.
+        clear Heqb Heqb0.
+        apply (f_equal (decode (A:=val))) in Heq.
+        rewrite !decode_encode in Heq. injection Heq as ->.
+        wp_pures.
+        iModIntro.
+        iSpecialize ("HΦ" with "[//]").
+        iExactEq "HΦ".
+        rewrite /vmap.val_def /=.
+        repeat f_equal.
+        rewrite /vmap.val_list_def /=.
+        change (v1, v)%V with ((λ x2 : val * val, let (a, b) := x2 in (a, b)%V) (v1, v)).
+        rewrite -fmap_cons. f_equal.
+        apply Sorted_unique.
+        { setoid_rewrite (merge_sort_Permutation). apply NoDup_fst_map_to_list. }
+        {
+          change (NoDup ((v1, v) :: x1).*1) with (NoDup ((v1, v2) :: x1).*1).
+          rewrite -Hl. setoid_rewrite (merge_sort_Permutation). apply NoDup_fst_map_to_list. }
+        { apply Sorted_merge_sort. apply _. }
+        {
+          lazymatch goal with [ H : merge_sort ?c ?l = ?l2 |- _ ] =>
+                                (pose proof Sorted_merge_sort (H:=(@vmap.cmp_dec ext)) c l) end.
+          rewrite Hl in H0.
+          inversion H0. subst.
+          econstructor.
+          { done. }
+          { inversion H4; econstructor. done. }
+        }
+        {
+          lazymatch goal with [ H : merge_sort ?c ?l = ?l2 |- _ ] =>
+                                (pose proof Sorted_merge_sort (H:=(@vmap.cmp_dec ext)) c l as Hs) end.
+          rewrite Hl in Hs.
+          setoid_rewrite merge_sort_Permutation.
+
+        }
+    }
+
 Admitted.
 
 End wps.
